Db/Backends/SqlExpr.lean
@@ -1,0 +1,58 @@
+/-
+Copyright (c) 2026 Christian Merten. All rights reserved.
+Released under Apache 2.0 license as described in the file LICENSE.
+Authors: Christian Merten
+-/
+
+namespace SQL
+
+inductive Expr where
+  | true
+  | false
+  | eq (e₁ e₂ : Expr)
+  | and (e₁ e₂ : Expr)
+  | var (table column : String)
+  | str (s : String)
+  | int (n : Int)
+  | null
+  deriving Repr
+
+def Expr.toString : Expr → String
+  | .true => "true"
+  | .false => "false"
+  | .eq e₁ e₂ => s!"({e₁.toString}) = ({e₂.toString})"
+  | .and e₁ e₂ => s!"({e₁.toString}) AND ({e₂.toString})"
+  | .var table column => s!"{table}.{column}"
+  | .str s => s!"'{s}'"
+  | .int n => ToString.toString n
+  | .null => "NULL"
+
+mutual
+
+inductive JoinType where
+  | inner
+  | outer
+
+inductive JoinConnect where
+  | onCondition (cond : Expr)
+  | usingColumn (column : String) (columns : List String)
+
+inductive From where
+  | tableName (name : String) (alias : String)
+  | select (sel : Select) (alias : String)
+  | join (left right : From) (joinType : JoinType) (connect : JoinConnect)
+  | naturalJoin (left right : From) (joinType : JoinType)
+  | crossJoin (left right : From)
+
+inductive Selector where
+  | all
+  | expressions (l : Expr) (alias : String)
+
+structure Select where
+  selector : List (Selector)
+  «from» : List From
+  «where» : Option Expr
+
+end
+
+end SQL
