Db/Interpretation/Basic.lean
@@ -7,18 +7,17 @@ import Db.Migration.Basic
 import Db.Migration.Recipe
 
 structure Interpretation (query : Type) where
-  fromQuery {d : Database} (names : Std.HashSet d.Name) (q : Query d names) : query
+  fromQuery {d : Database} (view : View d) (q : Query d view) : query
 
 -- TODO: Should also support logging operations for a custom error type
 /-- An interpretation monad on the database `d` provides lookup and modification operations. -/
 class DBMonad (d : Database) (m : Type → Type) where
   /-- Lookup the given query on the database. -/
-  lookup {names : Std.HashSet d.Name} (q : Query d names) :
-    m (Array (Std.DHashMap d.Name (fun d ↦ d.column.Value)))
+  lookup {view : View d} (q : Query d view) : m (Array view.Entry)
   /-- Insert the given data into the database. Return true if successful, false otherwise. -/
   insert {name : d.Index} (data : d.Insert name) : m Unit
   /-- Delete rows matching the expression. Return number of deleted rows. -/
-  delete (e : DBExpr d .bool) : m Nat
+  delete {view : View d} (e : DBExpr view .bool) : m Nat
 
 class DBMonadWithMigrations (m : Type → Type) where
   [dbMonad (d : Database) : DBMonad d m]
