Db/Utils/String.lean
@@ -1,0 +1,16 @@
+@[simp]
+theorem ToString.toString_string (s : String) : ToString.toString s = s :=
+  rfl
+
+@[simp]
+theorem String.dropPrefix?_append (s pat : String) :
+    (pat ++ s).dropPrefix? pat = s := by
+  sorry
+
+theorem String.dropPrefix?_append_of_ne (s : String) {pat t : String} (h : pat ≠ t) :
+    (t ++ s).dropPrefix? pat = none := by
+  sorry
+
+@[simp]
+theorem String.toString_toSlice (s : String) : s.toSlice.toString = s := by
+  sorry
